keccakf_avx2

proof/amd64/avx2/Keccakf1600_avx2.ec
@@ -3,7 +3,8 @@ require import AllCore IntDiv List.
 from Jasmin require import JModel.
 
 
-from CryptoSpecs require import FIPS202_SHA3 FIPS202_Keccakf1600.
+from CryptoSpecs require import FIPS202_SHA3 FIPS202_Keccakf1600 Keccak1600_arrays.
+
 require import Keccak1600_avx2.
 
 from JazzEC require import Keccak1600_Jazz.
@@ -64,20 +65,21 @@ qed.
 lemma keccakf1600_pround_avx2_ll: islossless M.__keccakf1600_pround_avx2 
 by islossless.
 
+
 hoare keccak_pround_avx2_h _a:
  M.__keccakf1600_pround_avx2 :
  state = _a /\ stavx2INV _a ==> res = stavx2_keccak_pround _a.
 proof.
-(*
 proc.
-time
+circuit.
+(*
 bdep 1792 1792 [_a] [state] [state] stavx2_keccak_pround stavx2INV.
 + move=> |> Hinv.
   rewrite stavx2_bvP allP => l.
   by rewrite mem_seq1.
 move => |> Hinv st.
 by rewrite !stavx2_bvP /=.
-*) admit.
+*)
 qed.
 
 lemma keccakf1600_avx2_ll': islossless M.__keccakf1600_avx2.
@@ -150,12 +152,59 @@ proof. by conseq keccakf1600_avx2_ll (keccakf1600_avx2_h _a). qed.
 
 lemma stavx2_pack_ll: islossless M.__stavx2_pack by islossless.
 
+
+from JazzEC require import WArray200.
+
+op sliceget25_64_256 (st: W64.t Array25.t) (offset: int) : W256.t = 
+ if 8 %| offset
+ then
+  WArray200.get256_direct (WArray200.init64 (fun i => st.[i])) (offset %/ 8)
+ else W256.bits2w (take 256 (drop offset (flatten (map W64.w2bits (to_list st))))).
+
+bind op [W64.t & W256.t & Array25.t] sliceget25_64_256 "asliceget".
+realize le_size by done.
+realize bvaslicegetP.
+move => /= arr offset; rewrite /sliceget25_64_256 /= => H k kb. 
+case (8%| offset) => /= *; last by smt(W256.get_bits2w).
+rewrite /get256_direct pack32E initiE 1:/# /= initiE 1:/# /= initiE 1:/# /=.
+rewrite nth_take 1,2:/# nth_drop 1,2:/#.
+rewrite (BitEncoding.BitChunking.nth_flatten false 64 _). 
++ rewrite allP => x /=; rewrite mapP => He; elim He;smt(W64.size_w2bits).
+rewrite (nth_map W64.zero []); 1: smt(Array25.size_to_list).
+by rewrite nth_mkseq 1:/# /= bits8E /= initiE /# /=.
+qed.
+
 hoare stavx2_pack_h _st:
  M.__stavx2_pack
  : st=_st ==> res = stavx2_from_st25 _st.
 proof.
 proc.
-admit (* BDEP *).
+proc change 2: { state <- state.[0 <- VPBROADCAST_4u64 st.[0]]; }.
+ auto => /> &m; congr; congr.
+ rewrite get64E pack8E.
+ apply W64.ext_eq => i Hi /=.
+ by rewrite initiE //= initiE 1:/# initiE 1:/# /= bits8E initiE 1:/# /= /#.
+proc change 3: { state <- state.[1 <- sliceget25_64_256 st (1*8*8)]; };
+ 1: by auto => /#.
+proc change 5: { state <- state.[3 <- sliceget25_64_256 st (6*8*8)]; };
+ 1: by auto => /#.
+proc change 7: { state <- state.[4 <- sliceget25_64_256 st (11*8*8)]; };
+ 1: by auto => /#.
+proc change 10: { state <- state.[5 <- sliceget25_64_256 st (16*8*8)]; };
+ 1: by auto => /#.
+proc change 14: { state <- state.[6 <- sliceget25_64_256 st (21*8*8)]; };
+ 1: by auto => /#.
+admit (* ?????
+circuit.
+
+tentativas de tornear/perceber problema...
+proc change 4: { t128_0 <- W2u64.zeroextu128 st.[5]; }.
+ admit.
+proc change 6: { t128_1 <- W2u64.zeroextu128 st.[10]; }.
+ admit.
+circuit.
+
+*).
 qed.
 
 phoare stavx2_pack_ph _st:
@@ -166,12 +215,75 @@ proof. by conseq stavx2_pack_ll (stavx2_pack_h _st). qed.
 
 lemma stavx2_unpack_ll: islossless M.__stavx2_unpack by islossless.
 
+op sliceset25_64_256 (st: W64.t Array25.t) (offset: int) (bv: W256.t) : W64.t Array25.t =
+ if 8%| offset
+ then
+  stwords
+   (WArray200.set256_direct (WArray200.init64 (fun i => st.[i])) (offset %/ 8) bv)
+ else
+   Array25.of_list
+    witness
+    (map W64.bits2w (chunk 64 (take offset (flatten (map W64.w2bits (to_list st)))
+     ++ w2bits bv
+     ++ drop (offset + 256) (flatten (map W64.w2bits (to_list st)))))).
+
+lemma size_flatten_W64_w2bits (a : W64.t list) :
+  (size (flatten (map W64.w2bits (a))))  =  64 * size a.
+proof.
+  rewrite size_flatten -map_comp /(\o) /=.
+  rewrite StdBigop.Bigint.sumzE /= StdBigop.Bigint.BIA.big_mapT /(\o) /=. 
+  rewrite StdBigop.Bigint.big_constz count_predT /#.
+qed.
+
+bind op [W64.t & W256.t & Array25.t] sliceset25_64_256 "asliceset".
+realize le_size by done.
+realize bvaslicesetP.
+move => arr offset bv H /= k kb; rewrite /sliceset25_64_256 /=. 
+case (8 %| offset) => /= *; last first.
++ rewrite of_listK.
+   rewrite size_map size_chunk 1:// !size_cat size_take. smt().
+    rewrite size_flatten_W64_w2bits size_to_list size_w2bits /= ifT 1:/#.
+    by rewrite size_drop 1:/# size_flatten_W64_w2bits size_to_list /#.
+  rewrite -(map_comp W64.w2bits W64.bits2w) /(\o). 
+  have := eq_in_map ((fun (x : bool list) => w2bits ((bits2w x))%W64)) idfun (chunk 64
+        (take offset (flatten (map W64.w2bits (to_list arr))) ++ w2bits bv ++
+         drop (offset + 256) (flatten (map W64.w2bits (to_list arr))))).
+  rewrite iffE => [#] -> * /=; 1: by smt(in_chunk_size W64.bits2wK).
+  rewrite map_id /= chunkK 1://;1: by rewrite !size_cat size_take;
+    by smt(size_take size_drop  W64.size_w2bits size_cat Array25.size_to_list size_flatten_W64_w2bits size_ge0). 
+  by rewrite !nth_cat !size_cat /=;
+     smt(nth_take nth_drop size_take size_drop  W64.size_w2bits size_cat Array25.size_to_list size_flatten_W64_w2bits size_ge0). 
+rewrite (nth_flatten _ 64); 1: by rewrite allP => i;rewrite mapP => He; elim He;smt(W64.size_w2bits).
+rewrite (nth_map W64.zero []); 1: smt(Array25.size_to_list).
+rewrite nth_mkseq 1:/# /= initiE 1:/# /= get64E pack8E initiE 1:/# /= initiE 1:/# /= /set256_direct.
+rewrite initiE 1:/# /=.
+case (offset <= k && k < offset + 256) => *; 1: by 
+  rewrite ifT 1:/#  get_bits8 /= 1,2:/# initiE // initiE //.
+rewrite ifF 1:/# initiE 1:/# /=.
+rewrite (nth_flatten _ 64); 1: by rewrite allP => i;rewrite mapP => He; elim He;smt(W64.size_w2bits).
+rewrite (nth_map W64.zero []); 1: smt(Array25.size_to_list).
+rewrite nth_mkseq 1:/# /= bits8E /= initiE /# /=.
+qed.
+ 
+
 hoare stavx2_unpack_h _st:
  M.__stavx2_unpack
  : state=_st ==> res = stavx2_to_st25 _st.
 proof.
 proc.
-admit (* BDEP *).
+proc change 3: { st <- sliceset25_64_256 st (1*8*8) state.[1]; };
+ 1: by auto => /#.
+proc change 11: { st <- sliceset25_64_256 st (6*8*8) t256_4; };
+ 1: by auto => /#.
+proc change 15: { st <- sliceset25_64_256 st (11*8*8) t256_4; };
+ 1: by auto => /#.
+proc change 18: { st <- sliceset25_64_256 st (16*8*8) t256_4; };
+ 1: by auto => /#.
+proc change 21: { st <- sliceset25_64_256 st (21*8*8) t256_4; };
+ 1: by auto => /#.
+admit (* ??? Exception thrown: EcLib.EcCircuits.MissingOpBody
+circuit.
+*).
 qed.
 
 phoare stavx2_unpack_ph _st:
